src/dafny/beacon/ForkChoiceTypes.dfy
@@ -1,0 +1,66 @@
+/*
+ * Copyright 2020 ConsenSys Software Inc.
+ *
+ * Licensed under the Apache License, Version 2.0 (the "License"); you may 
+ * not use this file except in compliance with the License. You may obtain 
+ * a copy of the License at http://www.apache.org/licenses/LICENSE-2.0
+ *
+ * Unless required by applicable law or agreed to in writing, software dis-
+ * tributed under the License is distributed on an "AS IS" BASIS, WITHOUT 
+ * WARRANTIES OR CONDITIONS OF ANY KIND, either express or implied. See the 
+ * License for the specific language governing permissions and limitations 
+ * under the License.
+ */
+
+include "../utils/Eth2Types.dfy"
+
+/**
+ *  Provide datatype for fork choice rule (and LMD-GHOST)
+ */
+module ForkChoiceTypes {
+
+    import opened Eth2Types
+
+    // Containers
+
+    /** 
+     *  A Checkpoint. 
+     *  
+     *  Checkpoints have a slot number that is a multiple of
+     *  SLOTS_PER_EPOCH and so only the multiplier `epoch` is needed.
+     *  The block that is associated with this epoch should have a slot
+     *  number that is epoch * SLOTS_PER_EPOCH.
+     *  
+     *  @link{https://benjaminion.xyz/eth2-annotated-spec/phase0/beacon-chain/#checkpoint}
+     *
+     *  @param  epoch   An `Epoch` index i.e. slot number multiple of SLOTS_PER_EPOCH.
+     *  @param  root    A (hash of a) block. 
+     */
+    datatype CheckPoint = CheckPoint(
+        epoch: Epoch,
+        root: Root        
+    )    
+
+     /** 
+     *  A vote ie. an AttestationData.  
+     *  
+     *  @link{https://benjaminion.xyz/eth2-annotated-spec/phase0/beacon-chain/#attestationdata}
+     *
+     *  @param  slot                A slot number.
+     *  @param  beacon_block_root   Block determined to be the head of the chain as per running 
+     *                              LMD-GHOST at that slot. 
+     *  @param  source              The source (why should it be justified?) checkpoint (FFG link).
+     *  @param  target              The target (why should it be justified) checkpoint (FFG link).
+     *
+     *  @note   As (source, target) forms a pair, they should probably be grouped together
+     *          say as a Link rather than provided separately. 
+     */
+    datatype AttestationData = AttestationData(
+        slot: Slot,
+        // index, CommitteeIndex, not used, should be the committee the validator belongs to.
+        // beacon_block_root: Root, 
+        source: CheckPoint,
+        target: CheckPoint        
+    )    
+
+}
